work on funcall Mutual induction scheme

Simu/Cor.v
@@ -26,8 +26,29 @@ Section PRESERVATION.
    
   (* Let ge := globalenv prog. *)
   Let tge := Clight.globalenv tprog.
+
+  Definition chunk_of_typ ty := AST.chunk_of_type (Ctypes.typ_of_type ty).
+  Definition pointer_of_node node := pointer_of (type_of_inst node).
+
+  Hypothesis TRANSL: translate prog main_node = Errors.OK tprog.
+  Hypothesis STEPS:
+    forall c (e: Clight.env),
+      In c prog ->
+      exists loc_f f,
+        Globalenvs.Genv.find_symbol tge.(Clight.genv_genv) (step_id c.(c_name)) = Some loc_f
+        /\ Maps.PTree.get (step_id c.(c_name)) e = None
+        /\ Globalenvs.Genv.find_funct_ptr tge.(Clight.genv_genv) loc_f = Some (Clight.Internal f)
+        /\ Clight.type_of_fundef (Clight.Internal f) =
+          Ctypes.Tfunction (Ctypes.Tcons (type_of_inst_p c.(c_name))
+                                         (list_type_to_typelist (map snd (nelist2list c.(c_input)))))
+                                         (snd c.(c_output))
+                                         AST.cc_default
+        /\ Coqlib.list_norepet (Clight.var_names (Clight.fn_params f) ++ Clight.var_names (Clight.fn_vars f))
+        /\ Clight.fn_body f = snd (translate_stmt None c.(c_name) c.(c_step))
+        /\ length f.(Clight.fn_params) = 1 + Nelist.length c.(c_input)  
+        /\ Forall (fun x => Ctypes.access_mode (snd x) = Ctypes.By_value (chunk_of_typ (snd x)))
+                 (f.(Clight.fn_params) ++ f.(Clight.fn_vars)).
   
-  Hypothesis TRANSL: translate prog main_node = Errors.OK tprog.    
   (* Hypothesis WF: well_formed prog. *)
   (* Hypothesis MAINNODE: find_class main_node prog = Some (c_main, cls_main). *)
 
@@ -37,9 +58,7 @@ Section PRESERVATION.
   (*   admit. *)
   (* Qed. *)
   
-  Definition chunk_of_typ ty := AST.chunk_of_type (Ctypes.typ_of_type ty).
-  Definition pointer_of_node node := pointer_of (type_of_inst node).
-  
+    
   (* Definition main_fun := *)
   (*   Clight.mkfunction Ctypes.type_int32s AST.cc_default [] *)
   (*                     c_main.(c_vars) *)
@@ -107,79 +126,171 @@ Section PRESERVATION.
       stmt_eval prog S s1 S' ->
       well_formed_stmt c S' s2 ->
       well_formed_stmt c S (Comp s1 s2)
-  | wf_step: forall y ty clsid o es vs,
+  | wf_step: forall y ty c' prog' clsid o es vs me me' rv,
+      In (y, ty) c.(c_vars) ->
+      y <> self_id ->
+      In {| obj_inst := o; obj_class := clsid |} c.(c_objs) ->
+      find_class clsid prog = Some (c', prog') ->
       Nelist.Forall (well_formed_exp c) es ->
       Nelist.Forall2 (exp_eval S) es vs ->
-      Nelist.Forall2 (fun (e : exp) (v : val) => valid_val v (typeof e)) es vs ->
+      Nelist.Forall2 (fun e v => valid_val v (typeof e)) es vs ->
+      Nelist.Forall2 (fun e x => typeof e = snd x) es c'.(c_input) ->
+      ty = snd c'.(c_output) ->
+      find_inst o S me ->
+      stmt_step_eval prog me clsid vs me' rv ->
+      valid_val rv ty ->
       well_formed_stmt c S (Step_ap y ty clsid o es)
   | wf_skip: 
       well_formed_stmt c S Skip.
 
-  Definition compat_venv (c: class) (S: state) (env: Clight.env) (m: Memory.Mem.mem):  Prop :=
-    forall x v t,
-      find_var x S v ->
+  Definition compat_vars (c: class) (e: Clight.env) (m: Memory.Mem.mem): Prop :=
+    forall x t,
+      In c prog ->
       In (x, t) c.(c_vars) ->
       exists loc,
-        Maps.PTree.get x env = Some (loc, t)
-        /\ Memory.Mem.load (chunk_of_typ t) m loc 0 = Some v
-        /\ valid_val v t.
+        Maps.PTree.get x e = Some (loc, t)
+        /\ Memory.Mem.valid_access m (chunk_of_typ t) loc 0 Memtype.Writable.
 
-  Definition compat_menv (c: class) (S: state) (env: Clight.env) (m: Memory.Mem.mem):  Prop :=
-    forall x v t,
-      find_field x S v ->
+  Definition compat_self (c: class) (e: Clight.env) (m: Memory.Mem.mem): Prop :=
+    In c prog ->
+    exists co loc_self loc_struct ofs,
+      Maps.PTree.get self_id e = Some (loc_self, pointer_of_node c.(c_name))
+      /\ Memory.Mem.load AST.Mint32 m loc_self 0 = Some (Values.Vptr loc_struct ofs)
+      /\ Maps.PTree.get c.(c_name) tge.(Clight.genv_cenv) = Some co
+      /\ (forall x t,
+            In (x, t) c.(c_mems) ->
+            exists delta,
+              Ctypes.field_offset (Clight.genv_cenv tge) x (Ctypes.co_members co) = Errors.OK delta
+              /\ In (x, t) (Ctypes.co_members co)
+              /\ Memory.Mem.valid_access m (chunk_of_typ t) loc_struct (Int.unsigned (Int.add ofs (Int.repr delta))) Memtype.Writable)
+      /\ (forall o,
+            In o c.(c_objs) ->
+            exists delta,
+              Ctypes.field_offset (Clight.genv_cenv tge) o.(obj_inst) (Ctypes.co_members co) = Errors.OK delta).
+
+  (* Definition compat_fields (c: class) (e: Clight.env) (m: Memory.Mem.mem): Prop := *)
+  (*   forall x t co loc_self loc_struct ofs, *)
+  (*     In c prog -> *)
+  (*     In (x, t) c.(c_mems) -> *)
+  (*     Maps.PTree.get self_id e = Some (loc_self, pointer_of_node c.(c_name)) -> *)
+  (*     Memory.Mem.load AST.Mint32 m loc_self 0 = Some (Values.Vptr loc_struct ofs) -> *)
+  (*     Maps.PTree.get c.(c_name) tge.(Clight.genv_cenv) = Some co ->      *)
+  (*     exists delta, *)
+  (*       Ctypes.field_offset (Clight.genv_cenv tge) x (Ctypes.co_members co) = Errors.OK delta *)
+  (*       /\ In (x, t) (Ctypes.co_members co) *)
+  (*       /\ Memory.Mem.valid_access m (chunk_of_typ t) loc_struct (Int.unsigned (Int.add ofs (Int.repr delta))) Memtype.Writable. *)
+  
+  Definition compat_venv (c: class) (S: state) (e: Clight.env) (m: Memory.Mem.mem):  Prop :=
+    forall x v t loc,
+      In c prog ->
+      In (x, t) c.(c_vars) ->
+      Maps.PTree.get x e = Some (loc, t) ->
+      find_var x S v ->
+      Memory.Mem.load (chunk_of_typ t) m loc 0 = Some v
+      /\ valid_val v t.
+  
+  Definition compat_menv (c: class) (S: state) (e: Clight.env) (m: Memory.Mem.mem):  Prop :=
+    forall x v t co loc_self loc_struct ofs delta,
+      In c prog -> 
       In (x, t) c.(c_mems) ->
-      exists co loc' loc ofs delta,
-        Ctypes.field_offset (Clight.genv_cenv tge) x (Ctypes.co_members co) = Errors.OK delta
-        /\ Memory.Mem.load (chunk_of_typ t) m loc (Int.unsigned (Int.add ofs (Int.repr delta))) = Some v
-        /\ valid_val v t
-        /\ Maps.PTree.get c.(c_name) (Clight.genv_cenv tge) = Some co 
-        /\ Maps.PTree.get self_id env = Some (loc', pointer_of_node c.(c_name))
-        /\ Memory.Mem.load (chunk_of_typ (pointer_of_node c.(c_name))) m loc' 0 = Some (Values.Vptr loc ofs)
-        /\ Ctypes.access_mode (pointer_of_node c.(c_name)) = Ctypes.By_value (chunk_of_typ (pointer_of_node c.(c_name))).
-
+      find_field x S v ->
+      Maps.PTree.get self_id e = Some (loc_self, pointer_of_node c.(c_name)) ->
+      Memory.Mem.load AST.Mint32 m loc_self 0 = Some (Values.Vptr loc_struct ofs) ->
+      Maps.PTree.get c.(c_name) tge.(Clight.genv_cenv) = Some co ->
+      Ctypes.field_offset (Clight.genv_cenv tge) x (Ctypes.co_members co) = Errors.OK delta ->
+      Memory.Mem.load (chunk_of_typ t) m loc_struct (Int.unsigned (Int.add ofs (Int.repr delta))) = Some v
+      /\ valid_val v t.
+  
   Remark valid_val_implies_access:
     forall v t, valid_val v t -> Ctypes.access_mode t = Ctypes.By_value (chunk_of_typ t).
   Proof. introv H; apply H. Qed.
     
   Hint Constructors Clight.eval_lvalue Clight.eval_expr well_formed_stmt.
   Hint Resolve valid_val_implies_access.
+
+  Remark eval_var:
+    forall c S e le m x t v,
+      compat_vars c e m ->
+      compat_venv c S e m ->
+      In c prog ->
+      In (x, t) c.(c_vars) ->
+      find_var x S v ->
+      Clight.eval_expr tge e le m (Clight.Evar x t) v.
+  Proof.
+    introv Hvars Hvenv ? ? ?.
+    edestruct Hvars; eauto.
+    edestruct Hvenv; iauto.
+    eapply Clight.eval_Elvalue, Clight.deref_loc_value; iauto. 
+  Qed.
+
+  Remark evall_self_field:
+    forall c e le m x t co loc_self loc_struct ofs delta,
+      Maps.PTree.get self_id e = Some (loc_self, pointer_of_node (c_name c)) ->
+      Memory.Mem.load AST.Mint32 m loc_self 0 = Some (Values.Vptr loc_struct ofs) ->
+      Maps.PTree.get (c_name c) (Clight.genv_cenv tge) = Some co ->
+      Ctypes.field_offset (Clight.genv_cenv tge) x (Ctypes.co_members co) = Errors.OK delta ->
+      Clight.eval_lvalue tge e le m (deref_self_field c.(c_name) x t) loc_struct (Int.add ofs (Int.repr delta)).
+  Proof.
+    intros.
+    eapply Clight.eval_Efield_struct
+    with (id:=c.(c_name)) (att:=Ctypes.noattr); eauto.
+    eapply Clight.eval_Elvalue. 
+    - apply Clight.eval_Ederef. 
+      apply* Clight.eval_Elvalue.
+      apply* Clight.deref_loc_value.
+      reflexivity.
+    - apply* Clight.deref_loc_copy.
+  Qed.
+  
+  Remark eval_self_field:
+    forall c S e le m x t v,
+      compat_self c e m ->
+      compat_menv c S e m ->
+      In c prog ->
+      In (x, t) c.(c_mems) ->
+      find_field x S v ->
+      Clight.eval_expr tge e le m (deref_self_field c.(c_name) x t) v.
+  Proof.
+    introv Hself Hmenv ? Hin ?.
+    destruct* Hself as (? & ? & ? & ? & ? & ? & ? & Hmem & ?).  
+    specializes Hmem Hin; destruct_conjs.
+    edestruct Hmenv; eauto; destruct_conjs. 
+    eapply Clight.eval_Elvalue.
+    + apply* evall_self_field.
+    + apply* Clight.deref_loc_value.      
+  Qed.
   
   Lemma expr_eval_simu:
     forall c S exp v e le m,
+      compat_vars c e m ->
+      compat_self c e m ->
       compat_venv c S e m ->
       compat_menv c S e m ->
+      In c prog ->
       well_formed_exp c exp ->
       exp_eval S exp v ->
       Clight.eval_expr tge e le m (translate_exp c.(c_name) exp) v.
   Proof.
-    intros c S exp;
-    induction exp as [| |cst];
-    introv Hvenv Hmenv Hwf Heval;
-    inverts Heval; inverts Hwf; simpl.
+    intros c S exp; induction exp as [| |cst];
+    introv ? ? ? ? ? Hwf Heval; inverts Heval; inverts Hwf.
 
     (* Var x ty : "x" *)
-    - edestruct Hvenv; eauto.
-      eapply Clight.eval_Elvalue, Clight.deref_loc_value; iauto.
-
+    - apply* eval_var.
+      
     (* State x ty : "self->x" *)
-    - edestruct Hmenv; destruct_conjs; eauto.
-      eapply Clight.eval_Elvalue.
-      + eapply Clight.eval_Efield_struct
-        with (id:=c.(c_name)) (att:=Ctypes.noattr); eauto.
-        eapply Clight.eval_Elvalue. 
-        * apply Clight.eval_Ederef. 
-          eapply Clight.eval_Elvalue, Clight.deref_loc_value; eauto.
-        * apply* Clight.deref_loc_copy.
-      + apply* Clight.deref_loc_value.
-
+    - apply* eval_self_field.
+      
     (* Const c ty : "c" *)
     - destruct cst; constructor.
   Qed.
 
   Lemma exprs_eval_simu:
     forall c S es es' vs e le m,
+      compat_vars c e m ->
+      compat_self c e m ->
       compat_venv c S e m ->
       compat_menv c S e m ->
+      In c prog ->
       Nelist.Forall (well_formed_exp c) es ->
       Nelist.Forall2 (fun e v => valid_val v (typeof e)) es vs ->
       Nelist.Forall2 (exp_eval S) es vs ->
@@ -187,28 +298,10 @@ Section PRESERVATION.
       Clight.eval_exprlist tge e le m es' (list_type_to_typelist (map Clight.typeof es')) (nelist2list vs).
   Proof.
     Hint Constructors Clight.eval_exprlist.
-    introv Hvenv Hmenv Hwf Hvalid Hev Heq; subst es';
+    introv ? ? ? ? ? Hwf Hvalid Hev ?; subst es';
     induction Hev; inverts Hwf; inverts Hvalid; econstructor;
     (apply* expr_eval_simu || (rewrite type_pres; apply* sem_cast_same) || eauto).
   Qed.
-  
-  Definition compat_vars (c: class) (e: Clight.env) (m: Memory.Mem.mem): Prop :=
-    forall x t,
-      In (x, t) c.(c_vars) ->
-      exists loc,
-        Maps.PTree.get x e = Some (loc, t)
-        /\ Memory.Mem.valid_access m (chunk_of_typ t) loc 0 Memtype.Writable.
-
-  Definition compat_fields (c: class) (env: Clight.env) (m: Memory.Mem.mem): Prop :=
-    forall x t,
-      In (x, t) c.(c_mems) ->
-      exists co loc' loc ofs delta,
-        Ctypes.field_offset (Clight.genv_cenv tge) x (Ctypes.co_members co) = Errors.OK delta
-        /\ In (x, t) (Ctypes.co_members co)
-        /\ Maps.PTree.get c.(c_name) (Clight.genv_cenv tge) = Some co
-        /\ Maps.PTree.get self_id env = Some (loc', pointer_of_node c.(c_name))
-        /\ Memory.Mem.load (chunk_of_typ (pointer_of_node c.(c_name))) m loc' 0 = Some (Values.Vptr loc ofs)
-        /\ Memory.Mem.valid_access m (chunk_of_typ t) loc (Int.unsigned (Int.add ofs (Int.repr delta))) Memtype.Writable.
 
   Definition nodup_env (e: Clight.env) :=
     forall x x' loc t t',
@@ -278,21 +371,18 @@ Section PRESERVATION.
   Qed.
   
   Definition mem_sep (c: class) (e: Clight.env) (m: Memory.Mem.mem) :=
-    forall x loc t (* co x' *) ofs (* delta t' *) loc' (* v *) loc'',
+    forall x loc t loc_self loc_struct ofs,
       In (x, t) c.(c_vars) -> 
       Maps.PTree.get x e = Some (loc, t) ->
-      Maps.PTree.get self_id e = Some (loc'', pointer_of_node c.(c_name)) ->
-      (* Maps.PTree.get c.(c_name) (Clight.genv_cenv tge) = Some co -> *)
-      (* Ctypes.field_offset (Clight.genv_cenv tge) x' (Ctypes.co_members co) = Errors.OK delta -> *)
-      (* Memory.Mem.load (chunk_of_typ t') m loc' (Int.unsigned (Int.add ofs (Int.repr delta))) = Some v -> *)
-      Memory.Mem.load (chunk_of_typ (pointer_of_node c.(c_name))) m loc'' 0 = Some (Values.Vptr loc' ofs) ->
-      loc <> loc'.
+      Maps.PTree.get self_id e = Some (loc_self, pointer_of_node c.(c_name)) ->
+      Memory.Mem.load AST.Mint32 m loc_self 0 = Some (Values.Vptr loc_struct ofs) ->
+      loc <> loc_struct.
 
   Definition self_sep (c: class) (e: Clight.env) (m: Memory.Mem.mem) :=
-    forall loc ofs loc',
-      Maps.PTree.get self_id e = Some (loc', pointer_of_node c.(c_name)) ->
-      Memory.Mem.load (chunk_of_typ (pointer_of_node c.(c_name))) m loc' 0 = Some (Values.Vptr loc ofs) ->
-      loc <> loc'.
+    forall loc_self loc_struct ofs,
+      Maps.PTree.get self_id e = Some (loc_self, pointer_of_node c.(c_name)) ->
+      Memory.Mem.load AST.Mint32 m loc_self 0 = Some (Values.Vptr loc_struct ofs) ->
+      loc_struct <> loc_self.
 
   Definition fields_sep (m: Memory.Mem.mem) :=
     forall co x x' t t' ofs delta delta',
@@ -308,197 +398,6 @@ Section PRESERVATION.
          (BinInt.Z.add (Int.unsigned (Int.add ofs (Int.repr delta)))
                        (Memdata.size_chunk (chunk_of_typ t)))
          (Int.unsigned (Int.add ofs (Int.repr delta')))).
-        
-  Lemma compat_assign_pres:
-    forall c S env m loc x e v,
-      compat_venv c S env m ->
-      compat_menv c S env m ->
-      compat_vars c env m ->
-      compat_fields c env m ->
-      mem_sep c env m ->
-      self_sep c env m ->
-      nodup_env env ->
-      nodup_vars c ->
-      Maps.PTree.get x env = Some (loc, typeof e) ->
-      In (x, typeof e) c.(c_vars) ->
-      v = Values.Val.load_result (chunk_of_typ (typeof e)) v ->
-      valid_val v (typeof e) ->
-      x <> self_id ->
-      Memory.Mem.valid_access m (chunk_of_typ (typeof e)) loc 0 Memtype.Writable ->
-      exp_eval S e v ->
-      exists m', Memory.Mem.store (chunk_of_typ (typeof e)) m loc 0 v = Some m' 
-            /\ compat_venv c (update_var x S v) env m'
-            /\ compat_menv c S env m'
-            /\ compat_vars c env m' 
-            /\ compat_fields c env m' 
-            /\ mem_sep c env m'
-            /\ self_sep c env m'.
-  Proof.
-    intros ** Hvenv Hmenv Hvars Hfields Hsep Hself_sep Hnodupenv Hnodupvars Hget Hin Hloadres ? ? ? ?.
-    edestruct Memory.Mem.valid_access_store with (v:=v) as [m']; eauto. 
-    exists m'; splits*. 
-    - unfold compat_venv; intros x' v' t' Hfind Hin'.
-      destruct (AST.ident_eq x' x).
-      + subst x'.
-        apply find_update_var in Hfind; subst v'.
-        specializes Hnodupvars Hin Hin'; subst t'. 
-        exists loc; splits*.
-        rewrite Hloadres; apply* Memory.Mem.load_store_same.
-      + apply gso_var in Hfind; auto.
-        edestruct Hvenv as [loc' [? [Hload]]]; eauto.
-        exists loc'; splits*.
-        destruct (Values.eq_block loc' loc).
-        * subst loc'.
-          edestruct Hnodupenv; eauto. 
-        * rewrite <-Hload. 
-          apply* Memory.Mem.load_store_other.
-    - unfold compat_menv; intros x' v' t' Hmem Hin'.
-      edestruct Hmenv
-        as (co & loc'' & loc' & ofs & delta & ? & Hload & ? & ? & Hself' & Hloadptr & ?); eauto.
-      exists co loc'' loc' ofs delta; splits*. 
-      + destruct (Values.eq_block loc loc').
-        * edestruct Hsep with (2:=Hget); eauto; contradiction.
-        * rewrite <-Hload.
-          apply* Memory.Mem.load_store_other.
-      + destruct (Values.eq_block loc'' loc).
-        * subst loc''.
-          edestruct Hnodupenv with (2:=Hget); eauto.
-        * rewrite <-Hloadptr.
-          apply* Memory.Mem.load_store_other.
-    - unfold compat_vars; intros x' t' Hin'.
-      edestruct Hvars as (loc' & ? & ?); eauto.
-      exists loc'; split*.
-      apply* Memory.Mem.store_valid_access_1.
-    - unfold compat_fields; intros x' t' Hin'.
-      edestruct Hfields as (co & loc1' & loc1 & ofs & delta & ? & ? & ? & ? & Hload & ?); eauto. 
-      exists co loc1' loc1 ofs delta; splits*.
-      + destruct (Values.eq_block loc1' loc).
-        * subst loc1'.
-          edestruct Hnodupenv with (2:=Hget); eauto.
-        * rewrite <-Hload; apply* Memory.Mem.load_store_other.
-      + apply* Memory.Mem.store_valid_access_1.
-    - unfold mem_sep; intros x' loc1 t' ofs loc1' loc1'' Hin1 Hget1 Hself Hload.
-      apply* Hsep.
-      instantiate (1:=ofs).
-      destruct (Values.eq_block loc1'' loc).
-      + subst loc1''.
-        edestruct Hnodupenv with (2:=Hget); eauto.
-      + rewrite <-Hload; symmetry; apply* Memory.Mem.load_store_other.
-    - unfold self_sep; intros loc1 ofs loc1' Hself Hload.
-      apply* Hself_sep.
-      instantiate (1:=ofs).
-      destruct (Values.eq_block loc1' loc).
-      + subst loc1'.
-        edestruct Hnodupenv with (2:=Hget); eauto.
-      + rewrite <-Hload; symmetry; apply* Memory.Mem.load_store_other.
-  Qed.
-
-   Lemma compat_stassign_pres:
-    forall c S env m x e v co loc loc' ofs delta,
-      compat_venv c S env m ->
-      compat_menv c S env m ->
-      compat_vars c env m ->
-      compat_fields c env m ->
-      mem_sep c env m ->
-      self_sep c env m ->
-      fields_sep m ->
-      nodup_mems c ->
-      In (x, (typeof e)) (Ctypes.co_members co) ->
-      Ctypes.field_offset tge.(Clight.genv_cenv) x (Ctypes.co_members co) = Errors.OK delta ->
-      Maps.PTree.get c.(c_name) (Clight.genv_cenv tge) = Some co ->
-      Maps.PTree.get self_id env = Some (loc', pointer_of_node c.(c_name)) ->
-      Memory.Mem.load (chunk_of_typ (pointer_of_node c.(c_name))) m loc' 0 = Some (Values.Vptr loc ofs) ->
-      In (x, typeof e) c.(c_mems) ->
-      v = Values.Val.load_result (chunk_of_typ (typeof e)) v ->
-      valid_val v (typeof e) ->
-     Memory.Mem.valid_access m (chunk_of_typ (typeof e)) loc (Int.unsigned (Int.add ofs (Int.repr delta))) Memtype.Writable ->
-      exp_eval S e v ->
-      exists m',
-        Memory.Mem.store (chunk_of_typ (typeof e)) m loc (Int.unsigned (Int.add ofs (Int.repr delta))) v = Some m'
-        /\ compat_venv c S env m'
-        /\ compat_menv c (update_field x S v) env m'
-        /\ compat_vars c env m'
-        /\ compat_fields c env m'
-        /\ mem_sep c env m'
-        /\ self_sep c env m'.
-  Proof.
-    intros ** Hvenv Hmenv Hvars Hfields Hsep Hself_sep Hfields_sep Hnodupmems Hmembers Hoffset Hmain Hself Hloadptr Hin Hloadres ? ? ?.
-    edestruct Memory.Mem.valid_access_store with (v:=v) as [m']; eauto. 
-    exists m'; splits*.
-    - unfold compat_venv; intros x' v' t' Hmto Hin'.
-      edestruct Hvenv as (loc'' & Hget & Hload' & ?); eauto.
-      exists loc''; splits*.
-      destruct (Values.eq_block loc'' loc).
-      + edestruct Hsep with (1:=Hin'); eauto.
-      + rewrite <-Hload'.
-        apply* Memory.Mem.load_store_other.
-    - unfold compat_menv; intros x' v' t' Hmem Hin'.
-      destruct (AST.ident_eq x' x).
-      + subst x'.
-        apply find_update_field in Hmem; subst v'.
-        specializes Hnodupmems Hin Hin'; subst t'. 
-        exists co loc' loc ofs delta; splits*.
-        * rewrite Hloadres; apply* Memory.Mem.load_store_same.
-        *{ destruct (Values.eq_block loc' loc).
-           - edestruct Hself_sep; eauto.  
-           - rewrite <-Hloadptr.
-             apply* Memory.Mem.load_store_other.
-         }
-      + apply gso_field in Hmem; auto.
-        edestruct Hmenv
-          as (co' & loc1' & loc1 & ofs' & delta' & ? & Hload' & ? & Hmain1 & Hself1 & Hloadptr1 & ?); eauto. 
-        rewrite Hmain1 in Hmain; inverts Hmain. 
-        rewrite Hself1 in Hself; inverts Hself. 
-        rewrite Hloadptr1 in Hloadptr; inverts Hloadptr.
-        exists co loc' loc ofs delta'; splits*.
-        * rewrite <-Hload'. apply* Memory.Mem.load_store_other. 
-        *{ destruct (Values.eq_block loc' loc).
-           - edestruct Hself_sep; eauto. 
-           - rewrite <-Hloadptr1.
-             apply* Memory.Mem.load_store_other.
-         }
-    - unfold compat_vars; intros x' t' Hin'.
-      edestruct Hvars as (loc1' & ? & ?); eauto.
-      exists loc1'; split; auto.
-      apply* Memory.Mem.store_valid_access_1.
-    - unfold compat_fields; intros x' t' Hin'.
-      edestruct Hfields as (co' & loc1' & loc1 & ofs' & delta' & ? & ? & ? & Hself' & Hload & ?); eauto. 
-      exists co' loc1' loc1 ofs' delta'; splits*.
-      + destruct (Values.eq_block loc1' loc).
-        * subst loc1'.
-          rewrite Hself in Hself'; inverts Hself'. 
-          edestruct Hself_sep; eauto.
-        * rewrite <-Hload; apply* Memory.Mem.load_store_other.
-      + apply* Memory.Mem.store_valid_access_1.
-    - unfold mem_sep; intros x' loc1 t' ofs' loc1' loc1'' Hin1 Hget1 Hself' Hload.
-      apply* Hsep.
-      instantiate (1:=ofs').
-      destruct (Values.eq_block loc1'' loc).
-      + subst loc1''.
-        rewrite Hself in Hself'; inverts Hself'.
-        edestruct Hself_sep; eauto.  
-      + rewrite <-Hload; symmetry; apply* Memory.Mem.load_store_other.
-    - unfold self_sep; intros loc1 ofs' loc1' Hself' Hload.
-      apply* Hself_sep.
-      instantiate (1:=ofs').
-      destruct (Values.eq_block loc1' loc).
-      + subst loc1'.
-        rewrite Hself in Hself'; inverts Hself'. 
-        edestruct Hself_sep; eauto.  
-      + rewrite <-Hload; symmetry; apply* Memory.Mem.load_store_other.
-  Qed.
-
-Remark ifte_translate:
-    forall c temp (b: bool) s1 s2,
-      translate_stmt temp c.(c_name) (if b then s1 else s2) =
-      if b then (translate_stmt temp c.(c_name) s1) else (translate_stmt temp c.(c_name) s2).
-  Proof.
-    now destruct b.
-  Qed.  
-
-  Hint Constructors Clight.eval_lvalue Clight.eval_expr well_formed_stmt.
-  Hint Resolve expr_eval_simu Clight.assign_loc_value sem_cast_same.
-  Hint Constructors well_formed_stmt.
 
   Definition c_state := (Clight.env * Clight.temp_env * Memory.Mem.mem)%type.
    
@@ -510,7 +409,7 @@ Remark ifte_translate:
       
       (* Clight state well defined *)
       compat_vars c e m ->
-      compat_fields c e m ->
+      compat_self c e m ->
 
       (* Clight side separation *)
       mem_sep c e m ->
@@ -524,56 +423,398 @@ Remark ifte_translate:
       match_states_bigbig c S (e, le, m).
 
   Hint Constructors match_states_bigbig.
-
-  Definition empty_temp_env: Clight.temp_env := Maps.PTree.empty val.
-      
-  Inductive unique_temp: Clight.temp_env -> option (ident * typ) -> Prop :=
-  | unique_empty:
-      unique_temp empty_temp_env None
-  | unique_singleton: forall le x v ty,
-      Maps.PTree.elements le = [(x, v)] -> 
-      unique_temp le (Some (x, ty)).
   
-  Theorem simu_bigbig:
-    forall c S1 s S2,
-      well_formed_stmt c S1 s ->
-      stmt_eval prog S1 s S2 ->
-      forall e1 le1 m1 temp,
-        (* unique_temp le1 temp -> *)
-        match_states_bigbig c S1 (e1, le1, m1) ->
-        exists le2 m2 t,
-          ClightBigstep.exec_stmt tge e1 le1 m1
-                                  (snd (translate_stmt temp c.(c_name) s))
-                                  t le2 m2 ClightBigstep.Out_normal
-          /\ match_states_bigbig c S2 (e1, le2, m2).
+  Remark load_same:
+    forall env x t x' t' m m' chk loc loc' v vptr vptr',
+      nodup_env env ->
+      x <> x' ->
+      Maps.PTree.get x env = Some (loc, t) ->
+      Maps.PTree.get x' env = Some (loc', t') ->
+      Memory.Mem.store chk m loc 0 v = Some m' ->
+      Memory.Mem.load AST.Mint32 m loc' 0 = Some vptr ->
+      Memory.Mem.load AST.Mint32 m' loc' 0 = Some vptr' ->
+      vptr' = vptr.
   Proof.
-    Check stmt_eval_ind_2.
-    clear TRANSL; introv WF EV; remember prog;
-    induction EV (* using stmt_eval_ind_2 with *)
-    (* (P := fun p St1 stmt St2 => *)
-    (*         well_formed_stmt c St1 stmt -> *)
-    (*         p = prog -> *)
-    (*         forall e1 le1 m1, *)
-    (*           match_states_bigbig c St1 (e1, le1, m1) -> *)
-    (*           exists le2 m2 t, *)
-    (*             ClightBigstep.exec_stmt tge e1 le1 m1 *)
-    (*                                     (snd (translate_stmt None c.(c_name) stmt)) *)
-    (*                                     t le2 m2 ClightBigstep.Out_normal *)
-    (*             /\ match_states_bigbig c St2 (e1, le2, m2) *)
-    (* ) *)
-    (*   (P0 := fun p me clsid vs me' rv => *)
-    (*            forall p' c S1 s S2, *)
-    (*              well_formed_stmt c S1 s -> *)
-    (*              stmt_eval p' S1 s S2 -> *)
-    (*              forall e1 le1 m1, *)
-    (*                match_states_bigbig c S1 (e1, le1, m1) -> *)
-    (*                exists le2 m2 t, *)
-    (*                  ClightBigstep.exec_stmt tge e1 le1 m1 *)
-    (*                                          (snd (translate_stmt None c.(c_name) s)) *)
-    (*                                          t le2 m2 ClightBigstep.Out_normal *)
-    (*                  /\ match_states_bigbig c S2 (e1, le2, m2)) *)
-    ; introv (* UNI *) MS;  try inverts WF;
-    inverts MS as Hvenv Hmenv Hvars Hfields.
+    introv Hnodupenv ? ? ? ? Hload Hload'.
+    destruct (Values.eq_block loc loc').
+      + subst loc.
+        edestruct Hnodupenv; eauto.
+      + assert (Memory.Mem.load AST.Mint32 m' loc' 0 = Memory.Mem.load AST.Mint32 m loc' 0)
+          as Eq by apply* Memory.Mem.load_store_other.
+        rewrite Eq in Hload'; rewrite Hload' in Hload; inverts Hload.
+        reflexivity.        
+  Qed.
+  
+  Lemma compat_assign_pres:
+    forall c S e le m loc x t exp v,
+      In c prog ->
+      match_states_bigbig c S (e, le, m) ->
+      Maps.PTree.get x e = Some (loc, t) ->
+      In (x, t) c.(c_vars) ->
+      v = Values.Val.load_result (chunk_of_typ t) v ->
+      valid_val v t ->
+      x <> self_id ->
+      exp_eval S exp v ->
+      exists m', Memory.Mem.store (chunk_of_typ t) m loc 0 v = Some m' 
+            /\ match_states_bigbig c (update_var x S v) (e, le, m').
+  Proof.
+    introv ? MS Hget Hin Hloadres ? ? ?.
+    inverts MS as Hvenv Hmenv Hvars Hself Hsep Hself_sep Hfields_sep Hnodupenv;
+      introv Hnodupvars Hnodupmems.
+    edestruct Hvars as (loc' & Hget' & ?); eauto.
+    rewrite Hget' in Hget; inverts Hget; rename Hget' into Hget.
+    edestruct Memory.Mem.valid_access_store with (v:=v) as [m']; eauto.
+    destruct* Hself as (co & loc_self & loc_struct & ofs & Hget_self & Hload_self & Hget_co & Hmem & ?).
+    exists m'; split*; constructor*.
+
+    - unfold compat_venv; intros x' v' t' loc' ? Hin' Hget' Hfind.
+      destruct (AST.ident_eq x' x).
+      + subst x'.
+        apply find_update_var in Hfind; subst v'.
+        specializes Hnodupvars Hin Hin'; subst t'. 
+        split*.
+        destruct (Values.eq_block loc' loc) as [|Neq].
+        * subst loc'.
+          rewrite Hloadres; apply* Memory.Mem.load_store_same.
+        * rewrite Hget in Hget'; inverts Hget'. now contradict Neq. 
+      + apply gso_var in Hfind; auto.
+        edestruct Hvenv as (Hload); eauto.
+        split*.
+        destruct (Values.eq_block loc' loc).
+        * subst loc'.
+          edestruct Hnodupenv; eauto. 
+        * rewrite <-Hload. 
+          apply* Memory.Mem.load_store_other.
+
+    - unfold compat_menv;
+      introv ? ? ? Hget_self' Hload_self' Hget_co' ?.
+      rewrite Hget_self' in Hget_self; inverts Hget_self.
+      rewrite Hget_co' in Hget_co; inverts Hget_co.
+      edestruct Hmenv as (Hload); eauto.
+      split*.
+      forwards* Eq: load_same; inverts Eq.
+      destruct (Values.eq_block loc loc_struct).
+      + edestruct Hsep; eauto.
+      + rewrite <-Hload.
+        apply* Memory.Mem.load_store_other.
+
+    - unfold compat_vars; intros.
+      edestruct Hvars as (loc'); eauto.
+      exists loc'; split*.
+      apply* Memory.Mem.store_valid_access_1.
+
+    - unfold compat_self; intro.
+      exists co loc_self loc_struct ofs.
+      splits*.
+      + destruct (Values.eq_block loc_self loc).
+        * subst loc.
+          edestruct Hnodupenv; eauto.
+        * rewrite <-Hload_self.
+          apply* Memory.Mem.load_store_other.
+      + introv Hin'.
+        specializes Hmem Hin'; destruct Hmem as (delta).
+        exists delta; splits*.
+        apply* Memory.Mem.store_valid_access_1.
+
+    - unfold mem_sep; introv ? ? Hget_self' ?.
+      rewrite Hget_self' in Hget_self; inverts Hget_self.
+      forwards* Eq: load_same; inverts Eq.
+      apply* Hsep.
+
+    - unfold self_sep; introv Hget_self' ?.
+      rewrite Hget_self' in Hget_self; inverts Hget_self.
+      forwards* Eq: load_same; inverts Eq.
+      apply* Hself_sep.
+  Qed.
+
+  Remark load_same':
+    forall c env m m' chk loc' v ofs loc1 ofs1 loc2 ofs2,
+      self_sep c env m ->
+      Maps.PTree.get self_id env = Some (loc', pointer_of_node c.(c_name)) ->
+      Memory.Mem.store chk m loc1 ofs v = Some m' ->
+      Memory.Mem.load AST.Mint32 m loc' 0 = Some (Values.Vptr loc1 ofs1) ->
+      Memory.Mem.load AST.Mint32 m' loc' 0 = Some (Values.Vptr loc2 ofs2) ->
+      Values.Vptr loc1 ofs1 = Values.Vptr loc2 ofs2.
+  Proof.
+    introv Hself_sep ? ? Hload1 Hload2.
+    assert (Memory.Mem.load AST.Mint32 m' loc' 0 = Memory.Mem.load AST.Mint32 m loc' 0)
+      as Eq.
+    apply* Memory.Mem.load_store_other.
+    left; intro Eq; symmetry in Eq; revert Eq; apply* Hself_sep.
+    rewrite Eq in Hload2; rewrite Hload2 in Hload1; inverts Hload1.
+    reflexivity.
+  Qed.
+
+  Lemma compat_stassign_pres:
+    forall c S e le m x t exp v co loc_self loc_struct ofs delta,
+      In c prog ->
+      match_states_bigbig c S (e, le, m) ->
+      Ctypes.field_offset tge.(Clight.genv_cenv) x (Ctypes.co_members co) = Errors.OK delta ->
+      Maps.PTree.get c.(c_name) (Clight.genv_cenv tge) = Some co ->
+      Maps.PTree.get self_id e = Some (loc_self, pointer_of_node c.(c_name)) ->
+      Memory.Mem.load AST.Mint32 m loc_self 0 = Some (Values.Vptr loc_struct ofs) ->
+      In (x, t) c.(c_mems) ->
+      v = Values.Val.load_result (chunk_of_typ t) v ->
+      valid_val v t ->
+     Memory.Mem.valid_access m (chunk_of_typ t) loc_struct (Int.unsigned (Int.add ofs (Int.repr delta))) Memtype.Writable ->
+      exp_eval S exp v ->
+      exists m',
+        Memory.Mem.store (chunk_of_typ t) m loc_struct (Int.unsigned (Int.add ofs (Int.repr delta))) v = Some m'
+        /\ match_states_bigbig c (update_field x S v) (e, le, m').
+  Proof.
+    intros ** ? MS Hoffset Hget_co Hget_self Hload_self Hin Hloadres ? ? ?.
+    inverts MS as Hvenv Hmenv Hvars Hself Hsep Hself_sep Hfields_sep Hnodupenv;
+      introv Hnodupvars Hnodupmems.
+    edestruct Memory.Mem.valid_access_store with (v:=v) as [m']; eauto. 
+    exists m'; split*; constructor*.
+
+    - unfold compat_venv; intros ** loc ? ? ? ?. 
+      edestruct Hvenv as (Hload); eauto.  
+      split*.
+      destruct (Values.eq_block loc loc_struct).
+      + edestruct Hsep; eauto.
+      + rewrite <-Hload.
+        apply* Memory.Mem.load_store_other.
+
+    - unfold compat_menv. intros x' v' t' ? ? ? ? ? ? Hin' Hfind' Hget_self' Hload_self' Hget_co' Hoffset'.
+      rewrite Hget_self' in Hget_self; inverts Hget_self.
+      rewrite Hget_co' in Hget_co; inverts Hget_co.
+      forwards* Eq: load_same'; inverts Eq.
+      destruct (AST.ident_eq x' x).
+      + subst x'.
+        rewrite Hoffset' in Hoffset; inverts Hoffset.
+        apply find_update_field in Hfind'; subst v'.
+        specializes Hnodupmems Hin Hin'; subst t'. 
+        split*.
+        rewrite Hloadres; apply* Memory.Mem.load_store_same.
+      + apply gso_field in Hfind'; auto.
+        edestruct Hmenv as (Hload); eauto.
+        split*.
+        rewrite <-Hload; apply* Memory.Mem.load_store_other.
+
+    - unfold compat_vars; intros.
+      edestruct Hvars as (loc'); eauto.
+      exists loc'; split*.
+      apply* Memory.Mem.store_valid_access_1.
+
+    - unfold compat_self; intro.
+      exists co loc_self loc_struct ofs.
+      destruct* Hself as (? & ? & ? & ? & Hget_self' & Hload_self' & Hget_co' & Hmem & ?).
+      rewrite Hget_co' in Hget_co; inverts Hget_co.
+      rewrite Hget_self' in Hget_self; inverts Hget_self.
+      rewrite Hload_self' in Hload_self; inverts Hload_self.  
+      splits*.
+      + destruct (Values.eq_block loc_self loc_struct).
+        * edestruct Hself_sep; eauto.
+        * rewrite <-Hload_self'.
+          apply* Memory.Mem.load_store_other.
+      + introv Hin'.
+        specializes Hmem Hin'; destruct Hmem as (delta').
+        exists delta'; splits*.
+        apply* Memory.Mem.store_valid_access_1.    
+        
+    - unfold mem_sep; introv ? ? Hget_self' ?.
+      rewrite Hget_self' in Hget_self; inverts Hget_self.
+      forwards* Eq: load_same'; inverts Eq.
+      apply* Hsep.
+
+    - unfold self_sep; introv Hget_self' ?.
+      rewrite Hget_self' in Hget_self; inverts Hget_self.
+      forwards* Eq: load_same'; inverts Eq.
+      apply* Hself_sep.
+  Qed.
+  
+  Remark alloc_exists:
+    forall vars e m,
+      exists e' m',
+        Clight.alloc_variables tge e m vars e' m'.
+  Proof.
+    induction vars as [|(x, ty)].
+    - do 3 econstructor.
+    - intros.
+      destruct (Memory.Mem.alloc m 0 (Ctypes.sizeof (Clight.genv_cenv tge) ty)) eqn: Eq.
+      specialize (IHvars (Maps.PTree.set x (b, ty) e) m0).
+      destruct* IHvars as (? & ? & ?).
+      do 3 econstructor; eauto.
+  Qed.
+
+  Remark assign_loc_exists:
+    forall v ty m loc,
+      Ctypes.access_mode ty = Ctypes.By_value (chunk_of_typ ty) ->
+      Memory.Mem.valid_access m (chunk_of_typ ty) loc 0 Memtype.Writable ->
+      exists m',
+        Clight.assign_loc tge.(Clight.genv_cenv) ty m loc Int.zero v m'.
+  Proof.
+    introv ? Hvalid.
+    forwards (? & ?): Memory.Mem.valid_access_store Hvalid.
+    do 2 econstructor; eauto.
+  Qed.
+  
+  Remark bind_parameters_exists:
+    forall xs vs e m,
+      length xs = length vs ->
+      Forall (fun x => exists loc,
+                  Maps.PTree.get (fst x) e = Some (loc, snd x)
+                  /\ Memory.Mem.valid_access m (chunk_of_typ (snd x)) loc 0 Memtype.Writable
+                  /\ Ctypes.access_mode (snd x) = Ctypes.By_value (chunk_of_typ (snd x))) xs ->
+      exists m',
+        Clight.bind_parameters tge e m xs vs m'.
+  Proof.
+    induction xs as [|(x, ty)]; destruct vs; introv Hlengths Hparams; try discriminate.
+    - do 2 econstructor.
+    - inverts Hparams as (? & ? & Hvalid & Haccess) Hparams.  
+      forwards (m' & Hassign): (assign_loc_exists v) Haccess Hvalid.
+      edestruct IHxs with (m:=m') (e:=e); eauto.
+      + inversion_clear Hassign as [|? ? ? ? Haccess'].
+        *{ clear IHxs Hlengths. induction xs.
+           - constructor.
+           - inverts Hparams as (loc & ?).
+             constructor.
+             + exists loc; splits*.
+               apply* Memory.Mem.store_valid_access_1.
+             + apply* IHxs.
+         }
+        * rewrite Haccess' in Haccess; discriminate.
+      + do 2 econstructor; eauto. 
+  Qed.
+
+  Remark alloc_variables_implies:
+    forall vars e m e' m', 
+      Clight.alloc_variables tge e m vars e' m' ->
+      Forall (fun x => Ctypes.access_mode (snd x) = Ctypes.By_value (chunk_of_typ (snd x))) vars ->
+      Forall (fun x => exists loc,
+                  Maps.PTree.get (fst x) e' = Some (loc, snd x)
+                  /\ Memory.Mem.valid_access m' (chunk_of_typ (snd x)) loc 0 Memtype.Writable
+                  /\ Ctypes.access_mode (snd x) = Ctypes.By_value (chunk_of_typ (snd x))) vars.
+  Proof.
+    induction vars.
+    - constructor.
+    - introv Halloc Hforall.
+      inverts Halloc.
+      constructor.
+      + exists b1; splits*.
+        * admit.
+        *{ assert (Memory.Mem.valid_access m1 (chunk_of_typ (snd (id, ty))) b1 0 Memtype.Writable).
+           - eapply Memory.Mem.valid_access_freeable_any.
+             apply* Memory.Mem.valid_access_alloc_same.
+             + omega.
+             + simpl. admit.
+             + eapply BinInt.Z.divide_0_r.
+           - admit.
+         }
+        * inverts* Hforall.
+      + apply* IHvars.
+        inverts* Hforall.
+  Qed.
+
+  Remark forall_app:
+    forall A (P: A -> Prop) l1 l2,
+      Forall P (l1 ++ l2) -> Forall P l1 /\ Forall P l2.
+  Proof.
+    introv HForall; split; rewrite Forall_forall in *; introv Hin;
+    apply HForall; apply in_or_app; [left | right]; auto.
+  Qed.
+
+  Lemma compat_funcall_pres:
+    forall m f vargs,
+      Datatypes.length (Clight.fn_params f) = Datatypes.length vargs ->
+      Forall (fun x => Ctypes.access_mode (snd x) = Ctypes.By_value (chunk_of_typ (snd x))) (f.(Clight.fn_params) ++ f.(Clight.fn_vars)) ->
+      exists m1 e_fun m2,
+        Clight.alloc_variables tge Clight.empty_env m (f.(Clight.fn_params) ++ f.(Clight.fn_vars)) e_fun m1 
+        /\ Clight.bind_parameters tge e_fun m1 f.(Clight.fn_params) vargs m2.
+  Proof.
+    introv Hlengths Haccesses.
+    forwards (e_fun & m1 & Halloc):
+      (alloc_exists (f.(Clight.fn_params) ++ f.(Clight.fn_vars)) Clight.empty_env m).
+    exists m1 e_fun.
+    forwards* Hforall': alloc_variables_implies Halloc Haccesses.
+    forwards (Hforall & H'): forall_app Hforall'; clear Hforall' H'.
+    forwards* (m2 & ?): bind_parameters_exists Hlengths Hforall.
+  Qed.
+  
+  Remark type_pres':
+    forall c' c es,
+      Nelist.Forall2 (fun e x => typeof e = snd x) es c'.(c_input) ->
+      map Clight.typeof (nelist2list (Nelist.map (translate_exp c.(c_name)) es)) =
+      map snd (nelist2list c'.(c_input)).
+  Proof.
+    intros c'.
+    induction (c_input c'); introv Heq;
+    inversion_clear Heq as [? ? Hty|? ? ? ? Hty Hforall2]; simpl.
+    - rewrite type_pres, Hty; auto.
+    - f_equal.
+      + rewrite type_pres, Hty; auto.
+      + specializes IHn Hforall2; eauto.
+  Qed.
+  
+  (* Remark ifte_translate: *)
+  (*   forall c temp (b: bool) s1 s2, *)
+  (*     translate_stmt temp c.(c_name) (if b then s1 else s2) = *)
+  (*     if b then (translate_stmt temp c.(c_name) s1) else (translate_stmt temp c.(c_name) s2). *)
+  (* Proof. *)
+  (*   now destruct b. *)
+  (* Qed.   *)
+
+  Hint Constructors Clight.eval_lvalue Clight.eval_expr well_formed_stmt.
+  Hint Resolve expr_eval_simu Clight.assign_loc_value sem_cast_same.
+  Hint Constructors well_formed_stmt.
+
+
+  (* Definition empty_temp_env: Clight.temp_env := Maps.PTree.empty val. *)
+      
+  (* Inductive unique_temp: Clight.temp_env -> option (ident * typ) -> Prop := *)
+  (* | unique_empty: *)
+  (*     unique_temp empty_temp_env None *)
+  (* | unique_singleton: forall le x v ty, *)
+  (*     Maps.PTree.elements le = [(x, v)] ->  *)
+  (*     unique_temp le (Some (x, ty)). *)
+
+  Remark ne_Forall2_lengths:
+    forall A B (P: A -> B -> Prop) l1 l2,
+      Nelist.Forall2 P l1 l2 -> Nelist.length l1 = Nelist.length l2.
+  Proof.
+    induction l1, l2; introv HForall2; inverts* HForall2.
+    simpl; f_equal; apply* IHl1.
+  Qed.
+
+  Axiom match_step: ident -> Clight.function -> Prop.
+  Axiom match_params: nelist val -> list val -> Prop.
+
+  Theorem simu_bigbig:
+    (forall p S1 s S2,
+        stmt_eval p S1 s S2 ->
+        p = prog ->
+        forall c,
+          In c prog ->
+          forall (WF: well_formed_stmt c S1 s)
+            e1 le1 m1 
+            (MS: match_states_bigbig c S1 (e1, le1, m1))
+            temp,
+          exists le2 m2 t,
+            ClightBigstep.exec_stmt tge e1 le1 m1
+                                    (snd (translate_stmt temp c.(c_name) s))
+                                    t le2 m2 ClightBigstep.Out_normal
+            /\ match_states_bigbig c S2 (e1, le2, m2))
+    /\ (forall p me clsid vs me' rv,
+          stmt_step_eval p me clsid vs me' rv ->
+          p = prog ->
+          forall m f vargs, 
+            match_step clsid f ->
+            match_params vs vargs ->
+            exists m' t,
+              ClightBigstep.eval_funcall tge m (Clight.Internal f) vargs t m' rv
+        ).
+  Proof.
+    clear TRANSL.
+    apply stmt_eval_step_ind; intros; 
+      try inversion_clear WF as [|? ? ? Hin| | |? ? ? ? ? ? ? ? ? ? ? ? ? Hin Hfind Hwfs Hevs Hvalids Htypes|];
+      try inverts MS as Hvenv Hmenv Hvars Hself; substs; intros.    
+
+    (* clear TRANSL; introv IN EV WF; remember prog; *)
+    (* induction EV as [| | | |? ? ? ? ? ? ? ? ? ? ? ? ? Step_eval|];  *)
+    (* introv (* UNI *) MS; *)
+    (* inversion_clear WF as [|? ? ? Hin| | |? ? ? ? ? ? ? ? ? ? Hin Hfind Hwfs Hevs Hvalids Htypes|]; *)
+    (* inverts MS as Hvenv Hmenv Hvars Hself; substs.   *)
 
     (* Assign x e : "x = e" *)
     - app_exp_eval_det.
@@ -582,25 +823,21 @@ Remark ifte_translate:
       do 3 econstructor; split*.
       apply* ClightBigstep.exec_Sassign. 
       rewrite* type_pres. 
-      
+       
     (* AssignSt x e : "self->x = e"*)
     - app_exp_eval_det.
-      edestruct Hfields; eauto; destruct_conjs.
-      edestruct compat_stassign_pres; iauto.
+      pose proof Hself as Hself'.
+      destruct* Hself' as (? & ? & ? & ? & ? & ? & ? & Hmem & ?).
+      specializes Hmem Hin; destruct_conjs.    
+      edestruct compat_stassign_pres; iauto.      
       do 3 econstructor; split*.
       apply* ClightBigstep.exec_Sassign.
-      + eapply Clight.eval_Efield_struct
-        with (id:=c.(c_name)) (att:=Ctypes.noattr); eauto.
-        apply* Clight.eval_Elvalue.  
-        * apply Clight.eval_Ederef. 
-          apply* Clight.eval_Elvalue.
-          apply Clight.deref_loc_value with (chunk:=AST.Mint32); eauto.
-        * apply* Clight.deref_loc_copy.
+      + apply* evall_self_field. 
       + rewrite* type_pres.
         
     (* Ifte e s1 s2 : "if e then s1 else s2" *)
     - destruct b.
-      + edestruct IHEV with (le1:=le1) (temp:=temp) as (? & ? & ? & Step & ?); eauto. 
+      + edestruct H3 with (le1:=le1) (temp:=temp) as (? & ? & ? & Step & ?); eauto. 
         do 3 econstructor; split*.
         simpl; destruct (translate_stmt temp (c_name c) s1);
         destruct (translate_stmt o (c_name c) s2).
@@ -608,7 +845,7 @@ Remark ifte_translate:
         * erewrite type_pres, bool_val_ptr; eauto.
         * eauto.
       + simpl; destruct (translate_stmt temp (c_name c) s1) as [temp1].
-        edestruct IHEV with (le1:=le1) (temp:=temp1) as (? & ? & ? & Step & ?); eauto. 
+        edestruct H3 with (le1:=le1) (temp:=temp1) as (? & ? & ? & Step & ?); eauto. 
         do 3 econstructor; split*.
         destruct (translate_stmt temp1 (c_name c) s2).
         apply* ClightBigstep.exec_Sifthenelse.
@@ -616,90 +853,93 @@ Remark ifte_translate:
         * eauto.
           
     (* Comp s1 s2 : "s1; s2" *)
-    - subst prog0.
-      app_stmt_eval_det.
-      edestruct IHEV1 with (le1:=le1) (temp:=temp) ; destruct_conjs; eauto.
+    - app_stmt_eval_det.
+      edestruct H0 with (le1:=le1) (temp:=temp) ; destruct_conjs; eauto.
       simpl. destruct (translate_stmt temp (c_name c) s1) as [temp1].
       destruct (translate_stmt temp1 (c_name c) s2) eqn: E2.
-      edestruct IHEV2 with (temp:=temp1) as (? & ? & ? & Step & ?); destruct_conjs; eauto.
+      edestruct H2 with (temp:=temp1) as (? & ? & ? & Step & ?); destruct_conjs; eauto.
       do 3 econstructor; split*.
       apply* ClightBigstep.exec_Sseq_1.
       rewrite* E2 in Step.
 
     (* Step_ap y ty clsid o [e1; ... ;en] : "y = step_clsid (&o, e1, ... , en)" *)
-    - assert (loc_f: Values.block). admit.
-      assert (Globalenvs.Genv.find_symbol (Clight.genv_genv tge) (step_id clsid) = Some loc_f). admit.
-      assert (Maps.PTree.get (step_id clsid) e1 = None). admit.
-
-      assert (loc_self: Values.block). admit.
-      assert (Maps.PTree.get self_id e1 = Some (loc_self, pointer_of_node (c_name c))). admit.
-      assert (loc_struct: Values.block). admit.
-      assert (ofs: Int.int). admit.
-      assert (Memory.Mem.loadv AST.Mint32 m1 (Values.Vptr loc_self Int.zero) = Some (Values.Vptr loc_struct ofs)). admit.
-      assert (co: Ctypes.composite). admit.
-      assert (Maps.PTree.get (c_name c) (Clight.genv_cenv tge) = Some co). admit.
-      assert (delta: Z). admit.
-      assert (Ctypes.field_offset (Clight.genv_cenv tge) o (Ctypes.co_members co) = Errors.OK delta). admit.
-
-      assert (f: Clight.function). admit.
-      assert (Globalenvs.Genv.find_funct (Clight.genv_genv tge) (Values.Vptr loc_f Int.zero) = Some (Clight.Internal f)). admit.
-
-      assert (e': Clight.env). admit.
-      assert (m': Memory.Mem.mem). admit.
-      assert (Clight.alloc_variables tge Clight.empty_env m1 (Clight.fn_params f ++ Clight.fn_vars f) e' m'). admit.
-      assert (m'': Memory.Mem.mem). admit.
-      assert (Clight.bind_parameters tge e' m' (Clight.fn_params f) (Values.Vptr loc_struct (Int.add ofs (Int.repr delta)) :: nelist2list vs0) m''). admit.
-
-      inverts H1.
-      assert (well_formed_stmt cls
-                               (omenv, adds (nefst (c_input cls)) vs v_empty) 
-                               (c_step cls)) as Hwf. admit.
-      assert (match_states_bigbig cls
-                                  (omenv, adds (nefst (c_input cls)) vs v_empty) 
-                                  (e', Clight.create_undef_temps (Clight.fn_temps f), m'')) as Hms. admit.
-      assert (Clight.fn_body f = snd (translate_stmt None (c_name cls) (c_step cls))) as Htr. admit.
+    - app_exps_eval_det.
+      app_find_inst_det.
+      app_stmt_step_eval_det.
       
-        do 3 econstructor; split*.
+      (* get the Clight corresponding function *)
+      forwards* Hin': find_class_In Hfind.
+      specialize (STEPS _ e1 Hin').
+      destruct STEPS as (loc_f & f & ? & ? & ? & Htype_fun & ? & Htr & Hlengths & Haccesses); clear STEPS.
+      forwards Eq: find_class_name Hfind.
+      rewrite Eq in *; clear Eq.
+      rewrite <-type_pres' with (c:=c) (es:=es) in Htype_fun; auto.
+
+      (* get the Clight corresponding field *)
+      pose proof Hself as Hself'.
+      destruct Hself' as (? & ? & loc_struct & ofs & ? & ? & ? & Hmem & Hobj); auto; clear Hmem.
+      specializes Hobj Hin; destruct Hobj as (delta).
+
+      (* get the Clight function entry state *)
+      forwards Eq1: ne_Forall2_lengths Htypes.
+      forwards Eq2: ne_Forall2_lengths Hvalids.
+      rewrite Eq2 in Eq1; clear Eq2.
+      rewrite <-Eq1 in Hlengths; clear Eq1.
+      assert (length f.(Clight.fn_params) =
+              length (Values.Vptr loc_struct (Int.add ofs (Int.repr delta)) :: nelist2list vs))
+        by (rewrite Hlengths; simpl; f_equal; rewrite Nelist.nelist2list_length; auto).
+      forwards* (m' & e' & m'' & ? & ?): (compat_funcall_pres m1). 
+
+      (* inverts Step_eval. *)
+
+      (* recursive funcall evaluation *)
+      edestruct H2 with
+      (f:=f) (vargs:=Values.Vptr loc_struct (Int.add ofs (Int.repr delta)) :: nelist2list vs);
+        destruct_conjs; eauto.
+      admit.
+      admit.
+           
+      do 3 econstructor; split~.
       eapply ClightBigstep.exec_Sseq_1.
-      + 
-        
-        eapply ClightBigstep.exec_Scall.
+
+      (* funcall: "$t = clsid_step(&(self->o), v1, ..., vn)" *)
+      + eapply ClightBigstep.exec_Scall; eauto.
         * simpl; eauto.
-        *{ eapply Clight.eval_Elvalue; simpl.
+        *{ eapply Clight.eval_Elvalue.
            - apply* Clight.eval_Evar_global.
            - apply* Clight.deref_loc_reference.
          }
         *{ econstructor.
            - eapply Clight.eval_Eaddrof.
-             eapply Clight.eval_Efield_struct
-             with (id:=c.(c_name)) (att:=Ctypes.noattr); eauto.
-             apply* Clight.eval_Elvalue.  
-             + apply Clight.eval_Ederef.
-               apply* Clight.eval_Elvalue.
-               apply Clight.deref_loc_value with (chunk:=AST.Mint32); eauto.
-             + apply* Clight.deref_loc_copy.                
+             apply* evall_self_field.
            - eapply sem_cast_same.
-             unfold valid_val. splits.
-             + reflexivity.
+             unfold valid_val; splits~.
              + discriminate.
-             + now simpl.
+             + simpl; trivial.
            - apply* exprs_eval_simu.
          }
         * eauto.
-        * admit.
-        *{ apply* ClightBigstep.eval_funcall_internal.
-           - admit.
-           - rewrite Htr.
-             (* specializes IHEV Hwf H22 Hms. *)
-             (* edestruct IHEV as (le2 & m2 & t & Hexec & Hms'); eauto. *)
-             skip.
-           - skip.
+
+      (* assignment: "y = $t" *)
+      + edestruct Hvars; eauto.
+        edestruct compat_assign_pres with (x:=y) (c:=c); iauto.
+        admit. skip.
+        eapply ClightBigstep.exec_Sassign; iauto. 
+        * eapply Clight.eval_Etempvar; eauto.
+          destruct temp; try destruct p; eapply Maps.PTree.gss. 
+        (* * eapply sem_cast_same. *)
+        (*   unfold valid_val; splits~. skip. *)
+        *{ econstructor.
+           - destruct* H10. 
            - skip.
          }
-      + skip.
-      + skip.
+      + constructor*.
+        admit.
 
     (* Skip : "skip" *)
     - do 3 econstructor; split*.
       eapply ClightBigstep.exec_Sskip.
+
+    (* funcall *)
+    - admit.
   Qed.
